coq/JsSyntaxAux.v
@@ -193,8 +193,7 @@ Qed.
 Global Instance prealloc_inhab : Inhab prealloc.
 Proof. apply (prove_Inhab prealloc_global). Qed.
 
-  (* LATER: use a plugin to generate definition *)
-  (* TODO: extract to ocaml primitive comparison *)
+  (* LATER: use a plugin to generate definitions *)
 
 Definition prealloc_compare bl1 bl2 :=
   match bl1, bl2 with
@@ -442,7 +441,7 @@ Definition mutability_compare m1 m2 : bool :=
 
 Global Instance mutability_comparable : Comparable mutability.
 Proof.
-  (* TODO: change proof script to follow the pattern of similar proofs above *)
+  (* NOTE: this proof script could be improved to follow the pattern of similar proofs above *)
   apply make_comparable. introv.
   applys decidable_make (mutability_compare x y).
   destruct x; destruct y; simpl; rew_refl;
@@ -982,80 +981,5 @@ Qed.
 
 
 (**************************************************************)
-(** Retrieve function and variable declarations from code *)
-
-(* TODO: move into JsPreliminary ? *)
-
-Definition element_funcdecl (el : element) : list funcdecl :=
-  match el with
-  | element_stat _ => nil
-  | element_func_decl name args bd =>
-      funcdecl_intro name args bd :: nil
-  end.
-
-Definition prog_funcdecl (p : prog) : list funcdecl :=
-  LibList.concat (LibList.map element_funcdecl (prog_elements p)).
-
-(* We follow the spec according to Sections 10.5 and 10.1.
-   10.5 tells us to fetch every variable declaration in the code.
-   10.1 tells us not to step inside function bodies. *)
-
-Fixpoint stat_vardecl (t : stat) : list string :=
-  match t with
-  | stat_expr _ => nil
-  | stat_label _ s => stat_vardecl s
-  | stat_block ts => LibList.concat (List.map stat_vardecl ts) (* Note: use List instead of LibList for fixpoint to be accepted *)
-  | stat_var_decl nes => LibList.map fst nes
-  | stat_if e s1 s2o => (stat_vardecl s1) ++
-                        (LibOption.unsome_default 
-                           nil
-                           (LibOption.map stat_vardecl s2o))
-  | stat_do_while _ s _ => stat_vardecl s
-  | stat_while _ _ s => stat_vardecl s
-  | stat_with _ s => stat_vardecl s
-  | stat_throw _ => nil
-  | stat_return _ => nil
-  | stat_break _ => nil
-  | stat_continue _ => nil
-  | stat_try s sco sfo => (stat_vardecl s) ++
-                          (LibOption.unsome_default 
-                             nil
-                             (LibOption.map 
-                                (fun x => stat_vardecl (snd x)) sco)) ++
-                          (LibOption.unsome_default 
-                             nil
-                             (LibOption.map stat_vardecl sfo))
-  | stat_for_in _ _ _ s => stat_vardecl s
-  | stat_for_in_var _ _ _ _ s => stat_vardecl s
-  | stat_debugger => nil
-  | stat_switch _ _ sb => switchbody_vardecl sb
-  end
-
-with switchbody_vardecl (sb : switchbody) : list string :=
-  match sb with
-  | switchbody_nodefault scl => LibList.concat (List.map switchclause_vardecl scl)
-  | switchbody_withdefault scl1 sl scl2 =>
-    (LibList.concat (List.map switchclause_vardecl scl1)) ++
-    (LibList.concat (List.map stat_vardecl sl)) ++
-    (LibList.concat (List.map switchclause_vardecl scl2))
-  end
-
-with switchclause_vardecl (sc : switchclause) : list string :=
-  match sc with
-  | switchclause_intro _ sl => LibList.concat (List.map stat_vardecl sl)
-  end.
-
-
-Definition element_vardecl (el : element) : list string :=
-  match el with
-  | element_stat t => stat_vardecl t
-  | element_func_decl name args bd => nil
-  end.
-
-Definition prog_vardecl (p : prog) : list string :=
-  LibList.concat (LibList.map element_vardecl (prog_elements p)).
-
-
-(**************************************************************)
-(** TODO: complete this file *)
+(** LATER: complete this file with the missing types. *)
 
